

9. Задача.

$$5) x_{n+1} - x_n = 2^{-n} \quad [x_n = x_0 + 2 \left(1 - \frac{1}{2^n}\right)]$$

$$\sum_{k=0}^{n-1} 2^{-k} = \frac{1 - \left(\frac{1}{2}\right)^n}{1 - \frac{1}{2}} = 2(1 - 2^{-n})$$

$$x_n = x_0 + 2(1 - 2^{-n})$$

$$x_{n+1} - x_n = 2(1 - 2^{-(n+1)}) - 2(1 - 2^{-n}) = 2[-2^{-(n+1)} + 2^{-n}] = 2 \cdot 2^{-n} = 2^{-n}$$

✓ проверка

$$6) x_{n+1} - x_n = 2x_n$$

рекуррентная формула с постоянным множителем

$$x_{n+1} = x_n + 2x_n = 3x_n$$

$$x_1 = 3x_0, \quad x_2 = 3x_1 = 3^2 x_0, \dots, x_n = 3^n x_0 \quad "x_n = 3^n x_0"$$

$$7) x_{n+1} = \frac{n+5}{n+3} x_n$$

$$x_n = x_0 \prod_{k=0}^{n-1} \frac{k+5}{k+3}$$

$$\prod_{k=0}^{n-1} \frac{k+5}{k+3}$$

$$[k+5] = (5)(6) \dots (n+4) = \frac{(n+4)!}{4!}$$

$$[k+3] = (3)(4) \dots (n+2) = \frac{(n+2)!}{2!}$$

$$\prod_{k=0}^{n-1} \frac{k+5}{k+3} = \frac{[n+4]! / 4!}{[n+2]! / 2!} = \frac{2! (n+4)!}{4! [n+2]!} = \frac{2!}{4!} = \frac{2}{24} = \frac{1}{12}$$

$$\frac{[n+4]!}{[n+2]!} = [n+4](n+3)$$

$$\prod_{k=0}^{n-1} \frac{k+5}{k+3} = \frac{[n+4](n+3)}{12}$$

$$x_n = x_0 \frac{[n+4](n+3)}{12}$$

$$8.) x_{n+1} = -x_n$$

$$x_1 = 0 \cdot x_0 = 0, x_2 = 1 \cdot x_1 = 0, \dots$$

$$x_2 = 1 \cdot x_1, x_3 = 2 \cdot x_2 = 2 \cdot 1 \cdot x_1, \dots, x_n = x_1 \prod_{k=1}^{n-1} k = x_1 (n-1)!$$

$$9.) x_{n+1} = -x_n$$

$$x_1 = -x_0, x_2 = -x_1 = (-1)^2 x_0, \dots, x_n = (-1)^n x_0$$

$$x_n = (-1)^n x_0$$

$$10.) 2x_{n+1} = x_n$$

$$x_{n+1} = \frac{1}{2} x_n \Rightarrow x_n = x_0 \left(\frac{1}{2}\right)^n = x_0 2^{-n}$$

$$11.) x_{n+1} = x_n + e^{-n}$$

$$x_n = x_0 + \sum_{k=0}^{n-1} e^{-k} = x_0 + \frac{1 + e^{-n}}{1 - e^{-1}}$$

$$x_n = 1 + \frac{1 + e^{-n}}{1 - e^{-1}}$$

$$12.) (n+1)x_{n+1} = (n+2)x_n \quad x_{n+1} = \frac{n+2}{n+1} x_n$$

$$x_n = x_0 \prod_{k=0}^{n-1} \frac{k+2}{k+1} = x_0 \frac{(n+1)!/1!}{n!0!} = x_0 (n+1)$$

$$13.) x_{n+1} + x_n = 2x_{n+2}$$

$$\overset{|n|}{x_{n+1}} = 3 \overset{|n|}{x_n} \Rightarrow \overset{|n|}{x_n} = C \cdot 3^n \quad p = 3p + 2 \Rightarrow -2p = 2 \Rightarrow p = -1$$

$$x_n = C \cdot 3^{-n} - 1 \quad "x_n = (x_0 + 1) 3^n - 1"$$

$$14.) x_{n+2} = x_n + x_{n+1}$$

$$r^2 + r - 1 = 0 \Rightarrow r_{1,2} = \frac{-1 \pm \sqrt{5}}{2}$$

$$x_n = k_1 \left(\frac{1 + \sqrt{5}}{2} \right)^n + k_2 \left(\frac{1 - \sqrt{5}}{2} \right)^n$$

$$1.) a) x_n = x_{n+1} + x_{n+3} \quad \text{нопарок 3.}$$

$$b) x_{n+1} = (x_n)^2 + (x_{n-1})^3 \quad \text{нопарок 1.}$$

$$b) \cancel{x_{n+2} + 4x_{n+1}} x_n + n x_{n-1} = n^2 \quad \text{нопарок 1}$$

$$2) x_{n+2} + 4x_{n+1} + 4x_n = 2^n \quad \text{нопарок 2}$$

$$g) x_{n+1} = x_n + 1 \quad \text{нопарок 1}$$

$$e) x_{n+1} = x_n + 1 \quad \text{нопарок 3}$$

$$a) 3; \quad b) 1; \quad g) 1;$$

$$d) 2; \quad 2) 2; \quad e) 3;$$

$$2) \cancel{x_n} = \cancel{x_n} - \cancel{n}$$

$$x_n = n^2 + n$$

$$x_{n+1} = (n+1)^2 + (n+1) = n^2 + 3n + 2$$

$$x_n + 2n + 2 = (n^2 + n) + 2n + 2 = n^2 + 3n + 2$$

$$x_n + 2n + 2 = (n^2 + n + k + 2n + 2) = n^2 + 3n + 2 + k$$

Ответ: Да

$$3) x_2 = 3, x_3 = 5$$

$$x_2 = C\alpha^2 = 3$$

$$x_3 = C\alpha^3 = 5$$

$$\frac{x_3}{x_2} = \frac{C\alpha^3}{C\alpha^2} = \alpha = \frac{5}{3}$$

$$C = \frac{x_2}{\alpha^2} = \frac{3}{\left(\frac{5}{3}\right)^2} = \frac{3 \cdot 9}{25} = \frac{27}{25}$$

$$4) x_{n+1} = 1.25x_n \quad \text{1 шаг}$$

$$\text{Есть } x_0 = 1600$$

$$x_2 = 1.25^2 \cdot 1600 = 1.5625 \cdot 1600 = 2500$$

$$x_4 = 1.25^4 \cdot 1600 = 2.4414 \cdot 1600 = 3906.25$$

$$\rightarrow \text{Пример: а) } x_{n+1} = 1.25x_n, \text{ б) 1 шаг, в) } x_2 = 2500, x_4 = 3906$$

$$5) x_{n+1} - x_n = 2^{-n}$$

$$\sum_{k=0}^{n-1} 2^{-k} = \frac{1 - 2^{-n}}{1 - \frac{1}{2}} = 2(1 - 2^{-n})$$

$$x_{n+1} - x_n = 2^{-n}$$

$$x_n - x_0 = \sum_{k=0}^{n-1} 2^{-k}$$

$$x_n = x_0 + 2(1 - 2^{-n}) = x_0 + 2 - 2^{1-n}$$

$$x_n = x_0 + 2\left(1 - \frac{1}{2^n}\right)$$